wordarray: fixed corres proof for fold
Although the corres lemma is not as strong as what is was previously,
the proof is now more robust and so should not break as easily. This is
especially true in the case that more functions are callable by fold.

cogent/examples/wa_connect/WordArray_UpdCCorres.thy
@@ -797,14 +797,15 @@ High level:
       * BilbyFS, Ext2FS
 *)
 thm corres_def corres_app_concrete corres_app_abstract
-thm wordarray_fold_no_break_0'_def[simplified] hoare_add_K dispatch_t4'_def
+thm wordarray_fold_no_break_0'_def hoare_add_K dispatch_t4'_def
 
 abbreviation "mk_urecord xs \<equiv> URecord (map (\<lambda>x. (x, upd.uval_repr x)) xs)"
 definition "foldmap_measure i end \<equiv> unat end - unat i"
 definition "foldmap_bounds frm to len i e 
-  \<equiv> frm \<le> i \<and> e = min to len \<and> (frm < e \<longrightarrow> i < e) \<and> (\<not>(frm < e) \<longrightarrow> frm = i)"
-definition "foldmap_inv foldmap \<xi>' \<sigma> s' p frm i f acc obsv r res'
-  \<equiv> (\<exists>\<sigma>' res. foldmap \<xi>' \<sigma> p frm i f acc obsv r (\<sigma>', res) \<and> val_rel res res' \<and> (\<sigma>', s') \<in> state_rel)"
+  \<equiv> frm \<le> i \<and> e = min to len \<and> (frm < e \<longrightarrow> i \<le> e) \<and> ((\<not>(frm < e)) \<longrightarrow> frm = i)"
+definition "foldmap_inv foldmap \<xi>' \<sigma> p frm i f acc obsv r \<sigma>' res s' res'
+  \<equiv> foldmap \<xi>' \<sigma> p frm i f acc obsv r (\<sigma>', res) \<and> val_rel res res' \<and> (\<sigma>', s') \<in> state_rel"
+definition "foldmap_inv_stat obsv obsv' \<equiv> val_rel obsv obsv'"
 lemma state_rel_ex: 
   "\<exists>\<sigma>. (\<sigma>, s) \<in> state_rel"
   apply (clarsimp simp: state_rel_def heap_rel_def heap_rel_ptr_def heap_rel_ptr_w32_def)
@@ -816,6 +817,12 @@ lemma whileLoop_add_invI:
   assumes "\<lbrace> P \<rbrace> whileLoop_inv c b init I (measure M) \<lbrace> Q \<rbrace>!"
   shows "\<lbrace> P \<rbrace> whileLoop c b init \<lbrace> Q \<rbrace>!"
   by (metis assms whileLoop_inv_def)
+
+lemma validNF_select_UNIV:
+  "\<lbrace>\<lambda>s. \<forall>x. Q x s\<rbrace> select UNIV \<lbrace>Q\<rbrace>!"
+  apply (subst select_UNIV_unknown)
+  apply (rule validNF_unknown)
+  done
 
 lemma
   "cogent_function_val_rel f (sint FUN_ENUM_mul) \<Longrightarrow> 
@@ -832,23 +839,151 @@ lemma
 thm validNF_def valid_def no_fail_def
 
 lemma fold_dispatch_wp:
-  "\<lbrakk>wa_abs_typing_u (UWA (TPrim (Num t)) len arr) ''WordArray'' [TPrim (Num t)] s r w \<sigma>;
+  "\<lbrakk>proc_ctx_wellformed \<Xi>; upd.proc_env_matches_ptrs \<xi>0 \<Xi>;
+    wa_abs_typing_u (UWA (TPrim (Num U32)) len arr) ''WordArray'' [TPrim (Num U32)] (Boxed ReadOnly ptrl) r w \<sigma>;
+    \<sigma> p = option.Some (UAbstract (UWA (TPrim (Num U32)) len arr));
+    upd.uval_typing \<Xi> \<sigma> acc (TPrim (Num U32)) ra wa; upd.uval_typing \<Xi> \<sigma> obsv TUnit ro {};
+    wa \<inter> r = {}; wa \<inter> ro = {}; p \<notin> wa;
     (\<Xi>, [], [option.Some (foldmap_funarg_type ''wordarray_fold_no_break_0'')] \<turnstile> 
     (App f (Var 0)) : (foldmap_funret_type ''wordarray_fold_no_break_0''));
     \<forall>x x' \<sigma> s. val_rel x x' \<longrightarrow>
       update_sem_init.corres wa_abs_typing_u wa_abs_repr (Generated.state_rel wa_abs_repr) 
         (App f (Var 0)) (do ret <- dispatch_t4' f_num x'; gets (\<lambda>s. ret) od) 
         \<xi>0 [x] \<Xi> [option.Some (foldmap_funarg_type ''wordarray_fold_no_break_0'')] \<sigma> s\<rbrakk> \<Longrightarrow>
-    \<lbrace>\<lambda>sa. (a', n') = (a, n) \<and> (\<exists>x v. args = t3_C.elem_C_update (\<lambda>_. v) a \<and>
-          \<sigma> (arr + size_of_num_type t * n) = option.Some x \<and> val_rel x v) \<and>
-      foldmap_inv upd_wa_foldnb_bod \<xi>0 \<sigma> sa p frm n f acc obsv r_set (t3_C.acc_C args) \<and>
-      foldmap_bounds frm to len n e\<rbrace>
+    \<lbrace>\<lambda>sa. (a', n') = (a, n) \<and> n < e \<and>
+      (\<exists>\<sigma>' res x v. args = t3_C.elem_C_update (\<lambda>_. v) a \<and>
+        \<sigma>' (arr + size_of_num_type U32 * n) = option.Some x \<and> val_rel x v \<and>
+      foldmap_inv upd_wa_foldnb_bod \<xi>0 \<sigma> p frm n f acc obsv (ra \<union> ro) \<sigma>' res sa (t3_C.acc_C args)) \<and>
+      foldmap_bounds frm to len n e \<and> foldmap_inv_stat obsv (t3_C.obsv_C args)\<rbrace>
       dispatch_t4' f_num args 
-    \<lbrace>\<lambda>ret sb. foldmap_inv upd_wa_foldnb_bod \<xi>0 \<sigma> sb p frm (n + 1) f acc obsv r_set ret \<and>
-      foldmap_bounds frm to len (n + 1) e \<and>
+    \<lbrace>\<lambda>ret sb. (\<exists>\<sigma>' res.
+        foldmap_inv upd_wa_foldnb_bod \<xi>0 \<sigma> p frm (n + 1) f acc obsv (ra \<union> ro) \<sigma>' res sb ret) \<and>
+      foldmap_inv_stat obsv (t3_C.obsv_C args) \<and> foldmap_bounds frm to len (n + 1) e \<and> 
       foldmap_measure (n + 1) to < foldmap_measure n' to\<rbrace>!"
-  sorry
-thm corres_sum
+  apply (subst validNF_def)
+  apply (clarsimp simp: \<Xi>_def wordarray_fold_no_break_0_type_def abbreviated_type_defs)
+  apply (subst (asm) abbreviated_type_defs[symmetric])+
+  apply (subst (asm) wordarray_fold_no_break_0_type_def[symmetric])+
+  apply (subst (asm) \<Xi>_def[symmetric])+
+  apply (clarsimp simp: abbreviated_type_defs)
+  apply (rule conjI)
+   apply (subst valid_def)
+   apply (clarsimp simp: foldmap_inv_def)
+   apply (rename_tac sa ret sb \<sigma>' res x v)
+   apply (erule_tac x = "mk_urecord [x, res, obsv]" in allE)
+   apply (erule_tac x = args in allE)
+   apply clarsimp
+   apply (erule impE)
+    apply (subst val_rel_simp; simp add: foldmap_inv_stat_def)
+   apply (erule_tac x = \<sigma>' in allE)
+   apply (erule_tac x = sa in allE)
+   apply (clarsimp simp: corres_def val_rel_simp)
+   apply (frule_tac t = "TPrim (Num U32)" in upd_wa_foldnb_bod_preservation[rotated 2]; simp?; clarsimp?)
+   apply (rename_tac r' w')
+   apply (subgoal_tac "upd.matches_ptrs \<Xi> \<sigma>' [URecord [(UPrim (LU32 v), RPrim (Num U32)),
+      (UPrim (LU32 (t3_C.acc_C a)), RPrim (Num U32)), (obsv, upd.uval_repr obsv)]]
+      [option.Some (TRecord [(''elem'', TPrim (Num U32), Present), (''acc'', TPrim (Num U32), Present),
+        (''obsv'', TUnit, Present)] Unboxed)] (r' \<union> ro) w'")
+    apply (erule impE, blast)
+    apply clarsimp
+    apply (erule_tac x = ret in allE)
+    apply (erule_tac x = sb in allE)
+    apply clarsimp
+    apply (drule upd.preservation[where \<tau>s = "[]" and K = "[]", simplified]; simp?)
+    apply clarsimp
+    apply (rename_tac \<sigma>'' rb wb)
+    apply (clarsimp simp: foldmap_bounds_def)
+    apply (case_tac "frm < to \<and> frm < len"; clarsimp)
+    apply (frule wa_abs_typing_u_elims(5))
+    apply (erule_tac x = n in allE; clarsimp)
+    apply (frule_tac p = "arr + 4 * n" in valid_ptr_not_in_frame_same; simp?)
+     apply (drule_tac x = "arr + 4 * n" and S' = r in orthD2; simp?)
+     apply (drule_tac t = U32 in  wa_abs_typing_u_elims(2)[where \<tau>s = "[_]", simplified]; simp)
+     apply blast
+    apply clarsimp
+    apply (drule_tac t = U32 and arr = arr and len = len and r' = "UPrim (LU32 ret)" 
+      in upd_wa_foldnb_bod_step; simp?; clarsimp?)
+     apply (rule conjI)
+      apply (drule_tac p = p in readonly_not_in_frame; simp?)
+     apply (subst Int_Un_distrib2)+
+     apply clarsimp
+     apply (rule conjI)
+      apply (rule disjointI)
+      apply (frule_tac p = x and r = ra and w = wa in upd.uval_typing_valid(1)[rotated 1]; simp?)
+      apply clarsimp
+      apply (drule_tac p = y in readonly_not_in_frame; simp?)
+      apply (drule upd.uval_typing_pointers_noalias; blast)
+     apply (rule conjI)
+      apply (rule disjointI)
+      apply (frule_tac p = x and r = ro and w = "{}" in upd.uval_typing_valid(1)[rotated 1]; simp?)
+      apply clarsimp
+      apply (drule_tac p = y in readonly_not_in_frame; simp?)
+      apply blast
+     apply (rule disjointI)
+     apply (frule wa_abs_typing_u_elims(5))
+     apply clarsimp
+     apply (erule_tac x = i in allE; clarsimp)
+     apply (drule_tac p = "arr + 4 * i" in readonly_not_in_frame; simp?)
+     apply (drule wa_abs_typing_u_elims(2); clarsimp)
+     apply blast
+    apply (rule conjI)
+     apply (rule_tac x = \<sigma>'' in exI; simp)
+    apply (frule_tac a = n and k = to in less_is_non_zero_p1)
+    apply (drule unatSuc2; clarsimp simp: word_less_nat_alt word_le_nat_alt foldmap_measure_def)
+    apply linarith
+   apply (rule upd.matches_ptrs_some[where r' = "{}" and w' = "{}", simplified])
+    apply (rule upd.u_t_struct; simp?)
+    apply (rule upd.u_t_r_cons1[where r = "{}" and w = "{}", simplified]; simp?)
+     apply (rule upd.u_t_prim'; clarsimp)
+    apply (rule upd.u_t_r_cons1[where r' = ro and w' = "{}", simplified]; simp?)
+     apply (drule_tac u = obsv in upd.uval_typing_frame(1); simp?)
+      apply blast
+     apply (rule upd.u_t_r_cons1[where r' = "{}" and w' = "{}", simplified]; simp?)
+      apply (rule upd.u_t_r_empty)
+     apply (erule u_t_unittE; clarsimp)
+    apply (rule disjointI)
+    apply (frule_tac p = y and r = ro in upd.uval_typing_valid(1)[where w = "{}", simplified]; simp?)
+    apply clarsimp
+    apply (drule_tac p = y in readonly_not_in_frame; simp?)
+    apply (drule_tac x = y and S' = ro in orthD2; simp?)
+   apply (rule upd.matches_ptrs_empty[where \<tau>s = "[]", simplified])
+  apply (subst no_fail_def)
+  apply clarsimp
+  apply (clarsimp simp: foldmap_inv_def)
+  apply (rename_tac sa \<sigma>' res x v)
+  apply (erule_tac x = "mk_urecord [x, res, obsv]" in allE)
+  apply (erule_tac x = args in allE)
+  apply clarsimp
+  apply (erule impE)
+   apply (subst val_rel_simp; simp add: foldmap_inv_stat_def)
+  apply (erule_tac x = \<sigma>' in allE)
+  apply (erule_tac x = sa in allE)
+  apply (clarsimp simp: corres_def val_rel_simp)
+  apply (frule_tac t = "TPrim (Num U32)" in upd_wa_foldnb_bod_preservation[rotated 2]; simp?; clarsimp?)
+  apply (rename_tac r' w')
+  apply (erule_tac x = "r' \<union> ro" in allE)
+  apply (erule_tac x = w' in allE)
+  apply (rotate_tac -1)
+  apply (erule notE)
+  apply (rule upd.matches_ptrs_some[where r' = "{}" and w' = "{}", simplified])
+   apply (rule upd.u_t_struct; simp?)
+   apply (rule upd.u_t_r_cons1[where r = "{}" and w = "{}", simplified]; simp?)
+    apply (rule upd.u_t_prim'; clarsimp)
+   apply (rule upd.u_t_r_cons1[where r' = ro and w' = "{}", simplified]; simp?)
+    apply (drule_tac u = obsv in upd.uval_typing_frame(1); simp?)
+     apply blast
+    apply (rule upd.u_t_r_cons1[where r' = "{}" and w' = "{}", simplified]; simp?)
+     apply (rule upd.u_t_r_empty)
+    apply (erule u_t_unittE; clarsimp)
+   apply (rule disjointI)
+   apply (frule_tac p = y and r = ro in upd.uval_typing_valid(1)[where w = "{}", simplified]; simp?)
+   apply clarsimp
+   apply (drule_tac p = y in readonly_not_in_frame; simp?)
+   apply (drule_tac x = y and S' = ro in orthD2; simp?)
+  apply (rule upd.matches_ptrs_empty[where \<tau>s = "[]", simplified])
+  done
+
+
 lemma upd_C_wordarray_fold_no_break_corres':
   "\<lbrakk>i < length \<gamma>; val_rel (\<gamma> ! i) v'; \<Gamma>' ! i = option.Some (prod.fst (prod.snd (\<Xi> ''wordarray_fold_no_break_0'')));
    \<gamma> ! i = URecord fs; f = prod.fst (fs ! 3); upd.proc_env_matches_ptrs \<xi>0 \<Xi>;
@@ -894,30 +1029,133 @@ gets (\<lambda>s. x)
   apply clarsimp
   apply (rename_tac acc ra wa obsv ro wo)
   apply (subst unknown_bind_ignore)+
-  apply clarsimp
+  apply (clarsimp simp: join_guards)
   apply wp
       apply (clarsimp simp: unknown_bind_ignore split: prod.split)
       apply (rename_tac var e)
       apply (rule_tac M = "\<lambda>((_, i), _). foldmap_measure i (t5_C.to_C v')" and 
-      I = "\<lambda>(a, b) s. foldmap_inv upd_wa_foldnb_bod \<xi>0 \<sigma> s (ptr_val (t5_C.arr_C v'))
-          (t5_C.frm_C v') b (uvalfun_to_exprfun f) acc obsv (ra \<union> ro) (t3_C.acc_C a) \<and> 
-        foldmap_bounds (t5_C.frm_C v') (t5_C.to_C v') len b e" in whileLoop_add_invI; simp?)
+      I = "\<lambda>(a, b) s. (\<exists>\<sigma>' res. foldmap_inv upd_wa_foldnb_bod \<xi>0 \<sigma> (ptr_val (t5_C.arr_C v'))
+          (t5_C.frm_C v') b (uvalfun_to_exprfun f) acc obsv (ra \<union> ro) \<sigma>' res s (t3_C.acc_C a)) \<and>
+          foldmap_inv_stat obsv (t3_C.obsv_C a) \<and>
+          foldmap_bounds (t5_C.frm_C v') (t5_C.to_C v') len b e" in whileLoop_add_invI; simp?)
       apply (wp; clarsimp simp: unknown_bind_ignore split: prod.splits)
-           apply (rename_tac sa a n args a' n')
-           apply (rule_tac a = a in fold_dispatch_wp; simp?)
-            apply (clarsimp simp: \<Xi>_def wordarray_fold_no_break_0_type_def abbreviated_type_defs)
+          apply (rename_tac sa a n args a' n') thm fold_dispatch_wp
+          apply (rule_tac a = a and wa = wa and ra = ra and ro = ro and w = "{}" and r = r and
+            ptrl = undefined in fold_dispatch_wp[rotated 2]; simp?)
+             apply (subst (asm) upd.uval_typing.simps[of _ _ _ TUnit, simplified]; simp?)
+             apply (erule disjE; clarsimp?)+
+             apply (rule upd.u_t_unit)
+            apply (clarsimp simp: Int_Un_distrib2)
            apply (clarsimp simp: \<Xi>_def wordarray_fold_no_break_0_type_def abbreviated_type_defs)
-          apply wp
+          apply (clarsimp simp: \<Xi>_def wordarray_fold_no_break_0_type_def abbreviated_type_defs)
          apply wp
         apply wp
        apply clarsimp
+       apply (rename_tac args j \<sigma>' res)
+       apply (clarsimp simp: foldmap_bounds_def foldmap_inv_def)
+       apply (frule wa_abs_typing_u_elims(5))
+       apply (erule_tac x = j in allE; clarsimp)
+       apply (drule_tac acc = acc and obsv = obsv and rb = ra and wb = wa and rc = ro
+          in upd_wa_foldnb_bod_preservation; simp?; clarsimp?)
+        apply (erule u_t_unittE; clarsimp intro!: upd.u_t_unit)
+       apply (frule_tac p = "ptr_val (t5_C.arr_C v')" in valid_ptr_not_in_frame_same; simp?)
+       apply (drule_tac p = "arr + 4 * j" in valid_ptr_not_in_frame_same; simp?)
+        apply (subst (asm) Int_Un_distrib2; clarsimp)
+        apply (drule_tac x = "arr + 4 * j" and S = wa and S' = r in orthD2; simp?)
+        apply (drule wa_abs_typing_u_elims(2); clarsimp)
+        apply blast
+       apply (thin_tac "_ \<in> state_rel")
+       apply (rule conjI)
+        apply (rule_tac x = \<sigma>' in exI)
+        apply (rule_tac x = res in exI)
+        apply (rule_tac x = "UPrim x" in exI)
+        apply clarsimp
+        apply (clarsimp simp: state_rel_def heap_rel_def heap_rel_ptr_w32_meta heap_rel_ptr_meta)
+        apply (rotate_tac -1)
+        apply (drule_tac p = "Ptr(arr + 4 * j)" in all_heap_rel_ptrD; simp?)
+         apply (clarsimp simp: type_rel_simp)
+        apply (rule_tac x = "heap_w32 s (PTR(32 word) (arr + 4 * j))" in exI)
+        apply (drule_tac p = "t5_C.arr_C v'" in all_heap_rel_ptrD; simp?)
+         apply (clarsimp simp: type_rel_simp wa_abs_repr_def)
+        apply (clarsimp simp: val_rel_WordArray_u32_C_def ptr_add_def heap_simp mult.commute)
+       apply (clarsimp simp: state_rel_def heap_rel_def heap_rel_ptr_w32_meta heap_rel_ptr_meta)
+       apply (rotate_tac -1)
+       apply (drule_tac p = "Ptr(arr + 4 * j)" in all_heap_rel_ptrD; simp?)
+        apply (clarsimp simp: type_rel_simp)
+       apply (drule_tac p = "t5_C.arr_C v'" in all_heap_rel_ptrD; simp?)
+        apply (clarsimp simp: type_rel_simp wa_abs_repr_def)
+       apply (clarsimp simp: is_valid_simp heap_simp val_rel_WordArray_u32_C_def ptr_add_def mult.commute)
+      apply (rule conjI)
+       apply (erule u_t_primtE; clarsimp)
+      apply (rule conjI)
+       apply (erule u_t_unittE; clarsimp)
+      apply (rule conjI)
+       apply (drule wa_abs_typing_u_elims(5); simp)
+      apply (rule conjI)
+       apply (erule u_t_funafuntE; clarsimp)
+      apply (rename_tac x' j \<sigma>' res)
+      apply (rule_tac x = \<sigma>' in exI)
+      apply (rule_tac x = res in exI)
+      apply (clarsimp simp: foldmap_inv_def)
+      apply (rule_tac x = "TPrim (Num U32)" in exI)
+      apply (rule_tac x = TUnit in exI)
+      apply (rule_tac x = "''elem''" in exI)
+      apply (rule_tac x = "''acc''" in exI)
+      apply (rule_tac x = "''obsv''" in exI)
+      apply clarsimp
+      apply (rule_tac x = ra in exI)
+      apply (rule conjI)
+       apply (intro exI, assumption)
+      apply (rule_tac x = ro in exI)
+      apply (rule conjI)
+       apply (erule u_t_unittE; clarsimp intro!: upd.u_t_unit)
+      apply (unfold foldmap_bounds_def)
+      apply (erule conjE)+
+      apply (case_tac "t5_C.frm_C v' < e")
+       apply (erule impE, assumption)
+       apply (thin_tac "_ \<longrightarrow> _")
+       apply clarsimp
+       apply (case_tac "j < t5_C.to_C v'"; clarsimp)
+       apply (rule upd_wa_foldnb_bod_to_geq_len; simp?)
+      apply (erule impE, assumption)
+      apply (thin_tac "_ \<longrightarrow> _")
+      apply clarsimp
+      apply (erule upd_wa_foldnb_bod.elims; clarsimp)
+      apply (case_tac "t5_C.frm_C v' < t5_C.to_C v'"; subst upd_wa_foldnb_bod.simps; clarsimp)
+     apply wp
+    apply wp
+   apply (rule validNF_select_UNIV)
+  apply (clarsimp simp: foldmap_inv_stat_def)
+  apply (clarsimp simp: order.strict_implies_order)
+  apply (clarsimp simp: foldmap_inv_def state_rel_def heap_rel_def heap_rel_ptr_meta)
+  apply (frule_tac p = "t5_C.arr_C v'" in all_heap_rel_ptrD; simp?)
+   apply (clarsimp simp: type_rel_simp wa_abs_repr_def)
+  apply (clarsimp simp: is_valid_simp val_rel_WordArray_u32_C_def heap_simp)
+  apply (rule conjI; clarsimp)
+   apply (rule conjI)
+    apply (rule_tac x = \<sigma> in exI)
+    apply (rule_tac x = acc in exI)
+    apply clarsimp
+    apply (drule wa_abs_typing_u_elims(5))
+    apply (subst upd_wa_foldnb_bod.simps; clarsimp)
+    apply (rule conjI; clarsimp)
+    apply (rename_tac j)
+    apply (erule_tac x = j in allE; clarsimp)
+   apply (subst min_def)
+   apply (subst (asm) not_le[symmetric])+
+   apply (subst if_not_P; simp?)
+  apply (rule conjI)
+   apply (rule_tac x = \<sigma> in exI)
+   apply (rule_tac x = acc in exI)
+   apply clarsimp
+   apply (drule wa_abs_typing_u_elims(5))
+   apply (subst upd_wa_foldnb_bod.simps; clarsimp)
+   apply (rule conjI; clarsimp)
+   apply (rename_tac j)
+   apply (erule_tac x = j in allE; clarsimp)
+  apply (subst min_def)
+  apply (clarsimp simp: not_le)
+  done
 
-  oops
-  thm cogent_function_val_rel
-  find_theorems name:"add_inv"
-(*
-abbreviation "wordarray_foldnb_inv \<xi>' \<sigma> p frm i f acc obsv t to v
-  \<equiv> (\<lambda>(a, b) s. (\<exists>\<sigma> r. upd_wa_foldnb_bod \<xi>' ))"
-*)
 end (* of context *)
 end
